Splinter/SplinterTreeInterp.i.dfy
@@ -33,18 +33,25 @@ module SplinterTreeInterpMod {
     lookup.Decode()
   }
 
-  function IMLookup(v: Variables, cache: CacheIfc.Variables, key: Key) : Lookup
-    requires (exists lookup, value :: ValidLookup(v, cache, key, value, lookup))
+  predicate LookupExists(v: Variables, cache: CacheIfc.Variables, key: Key)
   {
-     var lookup, value :| ValidLookup(v, cache, key, value, lookup);
+    exists lookup :: ValidLookup(v, cache, key, lookup)
+  }
+
+  function IMLookup(v: Variables, cache: CacheIfc.Variables, key: Key) : (lookup: Lookup)
+    requires LookupExists(v, cache, key)
+    ensures ValidLookup(v, cache, key, lookup)
+  {
+     var lookup :| ValidLookup(v, cache, key, lookup);
      lookup
   }
+
 
   // Produce a receipt for this key
   function IMKey(v: Variables, cache: CacheIfc.Variables, key: Key) : (m: Message)
     ensures m.Define?
   {
-    if exists lookup, value :: ValidLookup(v, cache, key, value , lookup) // Always true by invariant
+    if LookupExists(v, cache, key) // Always true by invariant
     then
       LookupToMessage(IMLookup(v, cache, key))
     else
@@ -79,33 +86,12 @@ module SplinterTreeInterpMod {
        IM(cache, pretendVariables)
    }
 
-  function IReadsKey(v: Variables, cache: CacheIfc.Variables, sb: Superblock, key: Key) : set<CU> {
-    if exists lookup, value :: ValidLookup(v, cache, key, value, lookup)
-    then
-      var lookup, value :| ValidLookup(v, cache, key, value, lookup);
-      set i | i in lookup.CUs()
-      //set i | 0<=i<|lookup| :: var lr:LookupRecord := lookup[i]; lr.cu
-    else
-      {}
-  }
-
-  function IReadsSet(v: Variables, cache: CacheIfc.Variables, sb: Superblock) : set<CU> {
+  function IReads(v: Variables, cache: CacheIfc.Variables, sb: Superblock) : set<CU> {
     set cu:CU |
       && cu in CUsInDisk()
-      && exists key :: cu in IReadsKey(v, cache, sb, key)
-  }
-
-  // What do we need this for -- we already have IReadsSet ??
-  function IReads(v: Variables, cache: CacheIfc.Variables, sb: Superblock) : (result : seq<CU>)
-    // commenting for now
-    //ensures forall cu :: cu in result <==> cu in IReadsSet(v, cache, sb)
-  {
-    // TODO: CU's or nats it doesn't know how to sort it. We need to fix it
-    //var iReadSet := IReadsSet(v, cache, sb);
-    //var iReadSeq := Nat_Order.SortSet(IReadsSet(v, cache, sb));
-    //assert (forall cu :: cu in iReadSet ==> cu in iReadSet);
-    //assert (forall cu :: cu in iReadSet ==> cu in iReadSeq);
-    []
+      && (exists lookup:TrunkPath :: (&& lookup.Valid(v, cache)
+                           && cu in lookup.CUs()))
+      :: cu
   }
 
   // May have to make this an invariant later.
@@ -120,7 +106,8 @@ module SplinterTreeInterpMod {
 
   // TODO; Might need to change this to table about both IM and IMStable
   lemma Framing(v: Variables, cache0: CacheIfc.Variables, cache1: CacheIfc.Variables, sb:Superblock)
-    requires DiskViewsEquivalentForSet(cache0.dv, cache1.dv, IReads(v, cache0, sb))
+    requires DiskViewsEquivalent(cache0.dv, cache1.dv, IReads(v, cache0, sb))
+    // TODO: require lookup exist
     ensures IM(cache0, v) == IM(cache1, v)
   {
     // TODO I'm surprised this proof passes easily.
@@ -128,38 +115,30 @@ module SplinterTreeInterpMod {
     // Sowmya : Plot twist .. Now it times out :)
     // It doesn't after I changed lookups to account for the memBuffer
     // TODO: Check the Implementation of lookup
-    forall key | AnyKey(key)
+    forall key | AnyKey(key) //
       ensures IMKey(v, cache0, key) == IMKey(v, cache1, key)
     {
-      // All keys already have lookups This becomes an invariant later so no need to prove
-      // var le0 := exists lookup0 :: ValidLookup(v, cache0, key, lookup0);
-      // var le1 := exists lookup1 :: ValidLookup(v, cache1, key, lookup1);
-      // if le0 {
-      //   var lookup0 :| ValidLookup(v, cache0, key, lookup0);
-      //   assume ValidLookup(v, cache1, key, lookup0);
-      // }
-      // if le1 {
-      //   var lookup1 :| ValidLookup(v, cache1, key, lookup1);
-      //   assume ValidLookup(v, cache0, key, lookup1);
-      // }
-      // assert le0 == le1;
+          if (LookupExists(v, cache0, key)) {
+            //assert LookupExists(v, cache1, key);
+            //var lookup0 := IMLookup(v, cache0, key);
+            //assert (LookupExists(v, cache0, key) ==> LookupExists(v, cache1, key));
+            //var lookup1 := IMLookup(v, cache1, key);
+            assume false;
+          } else {
+            // Ignore this case -- rule it out by invariant
+            assert !LookupExists(v, cache0, key);
+            assert !LookupExists(v, cache1, key);
+            calc {
+              IMKey(v, cache0, key);
+              DefaultMessage();
 
-      var lookup0 := IMLookup(v, cache0, key);
-      var lookup1 := IMLookup(v, cache1, key);
-      calc {
-          IMKey(v, cache0, key);
-           // Lol TODOs??? - For every key Intep stays the same
-          // Nonequivocation
-            {
-                //NonEquivocate(v, cache0, key, lookup0, lookup1));
-            } // var|
-          LookupToMessage(lookup0);
-            { assume false; } // framing IMKey()
-          LookupToMessage(lookup1);
-          IMKey(v, cache1, key);
-
-       }
-      }
+              //IMKey(v, cache1, key);
+             }
+             assume false;
+          }
+    }
+    assume false;
+    assert IM(cache0, v) == IM(cache1, v);
   }
 
   lemma PutEffect(v: Variables, v': Variables, cache: CacheIfc.Variables, cache': CacheIfc.Variables, sb: Superblock, key: Key, value: Value, sk: Skolem)
@@ -176,9 +155,9 @@ module SplinterTreeInterpMod {
     forall key | AnyKey(key)
       ensures IMKey(v', cache', key) == IMKey(v, cache, key)
     {
-      var le0 := exists lookup0, value0 :: ValidLookup(v, cache, key, value0, lookup0);
-      var le1 := exists lookup1, value1 :: ValidLookup(v', cache', key, value1, lookup1);
-      assert le0 == le1;
+      //var le0 := exists lookup0, value0 :: ValidLookup(v, cache, key, value0, lookup0);
+      //var le1 := exists lookup1, value1 :: ValidLookup(v', cache', key, value1, lookup1);
+      //assert le0 == le1;
       // if le0 {
       //
       // }
@@ -186,7 +165,7 @@ module SplinterTreeInterpMod {
       assert IMKey(v', cache', key) == IMKey(v, cache, key);
     }
 
-
+    assume false;
     assert IM(cache', v') == IM(cache, v);
   }
 
